internal/examples/semantics/prims.go
@@ -1,0 +1,14 @@
+package semantics
+
+import (
+	"github.com/tchajed/goose/machine"
+	"sync"
+)
+
+func testLinearize() bool {
+	m := new(sync.Mutex)
+	m.Lock()
+	machine.Linearize()
+	m.Unlock()
+	return true
+}
